Add bounded morphism and invariance proposition

BML/Def.lean
@@ -139,4 +139,55 @@ example {M₁ M₂ : Model World Atom} {x y : World} :
 
 end Proposition
 
+section
+
+variable {World1 World2 Atom : Type}
+variable {M1 : Model World1 Atom} {M2 : Model World2 Atom}
+
+
+/-- Definition 2.10 -/
+class BoundedMorphism (f : World1 → World2) where
+  /- w and f(w) satisfy the same proposition letters -/
+  same_prop : ∀ w p, M1.v w p ↔ M2.v (f w) p
+
+  /- homomorphism -/
+  hom : ∀ w v, M1.r w v → M2.r (f w) (f v)
+
+  /- back condition -/
+  back : ∀ w v', M2.r (f w) v' → ∃ v, M1.r w v ∧ f v = v'
+
+
+/-- Proposition 2.14 -/
+lemma model_satisfaction_invariance_under_bounded_morphism
+  {f : World1 → World2}
+  (hf : BoundedMorphism (M1 := M1) (M2 := M2) f)
+  (w : World1)
+  (φ : Proposition Atom) :
+  Proposition.eval M1 w φ ↔ Proposition.eval M2 (f w) φ := by
+  induction φ generalizing w with
+  | atom p => exact hf.same_prop w p
+  | not φ ih => simp [Proposition.eval, ih]
+  | and φ₁ φ₂ ih₁ ih₂ => simp [Proposition.eval, ih₁, ih₂]
+  | diamond φ ih =>
+      constructor
+      · intro h
+        simp only [Proposition.eval, ih] at h
+        rcases h with ⟨v, hv, hφ⟩
+        have h' : M2.r (f w) (f v) := hf.hom w v hv
+        simp only [Proposition.eval]
+        use f v
+      · intro h
+        simp only [Proposition.eval] at h
+        rcases h with ⟨v', hv', hφ⟩
+        obtain ⟨v, hv, h_eq⟩ := hf.back w v' hv'
+        simp only [Proposition.eval]
+        use v
+        constructor
+        · exact hv
+        · specialize ih v
+          rw [← h_eq] at hφ
+          exact ih.mpr hφ
+
+end
+
 end BML
